Add the ghost state structure for the trace and the various tables for tracking terms that can be made public

cryptis/rel.v
@@ -1,11 +1,12 @@
 From mathcomp Require Import ssreflect.
 From stdpp Require Import gmap.
-From iris.algebra Require Import agree auth lib.gset_bij gmap list excl.
+From iris.algebra Require Import agree auth gset gmap list excl.
 From iris.algebra Require Import functions.
+From iris.algebra.lib Require Import gset_bij mono_list.
 From iris.base_logic.lib Require Import saved_prop invariants.
 From iris.heap_lang Require Import notation proofmode.
 From cryptis Require Import lib gmeta nown.
-From cryptis.core Require Import term minted.
+From cryptis.core Require Import term minted public.
 
 From reloc Require Import reloc.
 From cryptis.core Require Import minted_spec.
@@ -14,63 +15,99 @@ Set Implicit Arguments.
 Unset Strict Implicit.
 Unset Printing Implicit Defensive.
 
-Definition term_part_bijR := gset_bijUR term term.
-
-Class publicGpreS Σ := PublicGPreS {
-  publicGpreS_term_part_bij : inG Σ term_part_bijR;
-  publicGpreS_meta : metaGS Σ;
+Class public_relGpreS Σ := Public_relGpreS {
+  #[local] public_relGpreS_trace :: inG Σ (mono_listUR (term * term)%type);
+  #[local] public_relGpreS_pub :: inG Σ (gset_bijUR term term);
+  #[local] public_relGpreS_priv :: inG Σ (authUR (gset_disjUR (term * term)));
+  #[local] public_relGpreS_flow_l :: inG Σ (authUR (gset_disjUR (term *  term)));
+  #[local] public_relGpreS_flow_r :: inG Σ (authUR (gset_disjUR (term *  term)));
 }.
 
-Local Existing Instance publicGpreS_term_part_bij.
-Local Existing Instance publicGpreS_meta.
-
-Class publicGS Σ := PublicGS {
-  public_inG : publicGpreS Σ;
-  public_term_part_bij_name : gname;
+Class public_relGS Σ := Public_relGS {
+  #[local] public_rel_inG :: public_relGpreS Σ;
+  public_rel_trace_name  : gname;
+  public_rel_pub_name  : gname;
+  public_rel_priv_name  : gname;
+  public_rel_flow_l_name  : gname;
+  public_rel_flow_r_name  : gname;
 }.
 
-Global Existing Instance public_inG.
+Definition public_relΣ : gFunctors :=
+  #[GFunctor (authUR (gset_disjUR (term * term)));
+    GFunctor (authUR (gset_disjUR (term * term)));
+    GFunctor (authUR (gset_disjUR (term * term)));
+    GFunctor (mono_listUR (term * term)%type);
+    GFunctor (gset_bijUR term term)].
 
-Definition publicΣ : gFunctors :=
-  #[GFunctor term_part_bijR; metaΣ].
-
-Global Instance subG_publicGpreS Σ : subG publicΣ Σ → publicGpreS Σ.
+Global Instance subG_public_relGpreS Σ : subG public_relΣ Σ → public_relGpreS Σ.
 Proof. solve_inG. Qed.
+
+Implicit Types (tr: list (term * term)) (pub priv flow_l flow_r: gset (term * term)).
+Inductive dolev_yao tr : term -> term -> Prop :=
+  | dy_in t1 t2 : (t1, t2) ∈ tr -> dolev_yao tr t1 t2
+  | dy_int n : dolev_yao tr (TInt n) (TInt n)
+  | dy_pair t1a t1b t2a t2b : dolev_yao tr t1a t2a -> dolev_yao tr t1b t2b -> dolev_yao tr (TPair t1a t1b) (TPair t2a t2b)
+  | dy_fst t1a t1b t2a t2b : dolev_yao tr (TPair t1a t1b) (TPair t2a t2b) -> dolev_yao tr t1a t2a
+  | dy_snd t1a t1b t2a t2b : dolev_yao tr (TPair t1a t1b) (TPair t2a t2b) -> dolev_yao tr t1b t2b
+  | dy_hash t1 t2 : dolev_yao tr t1 t2 -> dolev_yao tr (THash t1) (THash t2)
+  | dy_key kt t1 t2 : dolev_yao tr t1 t2 -> dolev_yao tr (TKey kt t1) (TKey kt t2)
+  | dy_seal k1 k2 t1 t2 : dolev_yao tr k1 k2 -> dolev_yao tr t1 t2 -> dolev_yao tr (TSeal k1 t1) (TSeal k2 t2)
+  | dy_unseal k1 k2 t1 t1' t2 t2' : dolev_yao tr k1 k2 -> dolev_yao tr t1 t2 -> Spec.open k1 t1 = Some t1' -> Spec.open k2 t2 = Some t2' -> dolev_yao tr t1' t2'.
+
+Definition dolev_yao_consistent tr :=
+  (∀ t1 t1' t2 t2', dolev_yao tr t1 t1' -> dolev_yao tr t2 t2' ->
+    t1 = t2 <-> t1' = t2') ∧
+  (∀ t1 t2, dolev_yao tr t1 t2 -> Spec.to_int t1 = Spec.to_int t2) ∧
+  (∀ t1 t2, dolev_yao tr t1 t2 ->
+    is_Some (Spec.untuple t1) <-> is_Some (Spec.untuple t2)) ∧
+  (∀ t1 t1' t2 t2', dolev_yao tr t1 t1' -> dolev_yao tr t2 t2' ->
+    is_Some (Spec.open t1 t2) <-> is_Some (Spec.open t1' t2')) ∧
+  (∀ t1 t2, dolev_yao tr t1 t2 -> Spec.is_key t1 = Spec.is_key t2).
+
+Definition tables_consistent tr pub priv flow_l flow_r :=
+  (∀ t1 t2 t2', (t1, t2) ∈ pub → (t1, t2') ∈ priv → False) ∧
+  (∀ t1 t1' t2, (t1, t2) ∈ pub → (t1', t2) ∈ priv → False) ∧
+  (∀ t1 t2, (t1, t2) ∈ pub → dolev_yao tr t1 t2) ∧
+  (∀ t1 t1' t2, (t1, t2) ∈ priv → dolev_yao tr t1 t1' → False) ∧
+  (∀ t1 t2 t2', (t1, t2) ∈ priv → dolev_yao tr t1 t2' → False) ∧
+  (∀ t1 t1' t2 t2', (t1, t1') ∈ flow_l → (t1, t2) ∈ pub → (t1', t2') ∈ pub) ∧
+  (∀ t1 t1' t2 t2', (t2, t2') ∈ flow_r → (t1, t2) ∈ pub → (t1', t2') ∈ pub).
 
 Section Rel.
 
-Context `{!relocG Σ, !publicGS Σ}.
+Context `{!relocG Σ, !public_relGS Σ, !publicGS Σ}.
+
 Notation iProp := (iProp Σ).
 Notation iPropO := (iPropO Σ).
 Notation iPropI := (iPropI Σ).
 
-Implicit Types (k : senc_key) (t : term) (R : gset (term * term)).
+Definition public_rel_trace_auth (trace: list (term * term)) : iProp :=
+  own public_rel_trace_name (●ML trace).
 
-Definition enc_rel_auth t R : iProp :=
-  nown public_term_part_bij_name (nroot.@"enc".@t)
-    (gset_bij_auth (DfracOwn 1) R).
+Definition public_rel_pub_auth (pub: gset (term * term)) : iProp :=
+  own public_rel_pub_name (gset_bij_auth (DfracOwn 1) pub).
 
-Definition enc_rel_frag t t1 t2 : iProp :=
-  nown public_term_part_bij_name (nroot.@"enc".@t)
-    (gset_bij_elem t1 t2).
+Definition public_rel_priv_auth (priv: gset (term * term)) : iProp :=
+  own public_rel_priv_name (● (GSet priv)).
 
-Lemma enc_rel_alloc t1 t2 t R :
-  (∀ t2', (t1, t2') ∉ R) → (∀ t1', (t1', t2) ∉ R) →
-  enc_rel_auth t R ==∗
-  enc_rel_auth t ({[(t1, t2)]} ∪ R) ∗
-  enc_rel_frag t t1 t2.
-Proof.
-iIntros "%fresh1 %fresh2 own".
-iMod (nown_update with "own") as "own".
-apply: gset_bij_auth_extend => //=.
-iDestruct "own" as "[auth #frag]".
-rewrite -gset_op view_frag_op nown_op.
-iDestruct "frag" as "[#frag1 #frag2]".
-iModIntro. iFrame "#".
-iCombine "frag1 frag2" as "#frag".
-rewrite /enc_rel_auth /gset_bij_auth nown_op.
-by iFrame "#".
-Qed.
+Definition public_rel_flow_l_auth (flow_l: gset (term * term)) : iProp :=
+  own public_rel_flow_l_name (● (GSet flow_l)).
+
+Definition public_rel_flow_r_auth (flow_r: gset (term * term)) : iProp :=
+  own public_rel_flow_l_name (● (GSet flow_r)).
+
+Definition cryptis_rel_N := nroot .@ "cryptis_rel".
+
+(* to be addressed- probably should not have existentials *)
+Definition cryptis_rel_inv : iProp :=
+  ∃ tr pub priv flow_l flow_r,
+      public_rel_trace_auth tr ∗
+      public_rel_pub_auth pub ∗
+      public_rel_priv_auth priv ∗
+      public_rel_flow_l_auth flow_l ∗
+      public_rel_flow_r_auth flow_r ∗
+    ⌜dolev_yao_consistent tr ∧ tables_consistent tr pub priv flow_l flow_r⌝.
+
 
 Definition nonce_rel_auth R : iProp :=
   nown public_term_part_bij_name (nroot.@"nonce")
